Experiments/Maximal_Path_Trie.thy
@@ -873,7 +873,7 @@ subsection \<open>Removing Proper Prefixes From a Set of Sequences\<close>
 definition remove_proper_prefixes :: "'a list set \<Rightarrow> 'a list set" where
   "remove_proper_prefixes xs = {x . x \<in> xs \<and> (\<nexists> x' . x' \<noteq> [] \<and> x@x' \<in> xs)}"
 
-lemma remove_proper_prefixes[code] :
+lemma remove_proper_prefixes_code[code] :
   "remove_proper_prefixes (set xs) = (case xs of [] \<Rightarrow> {} | (x#xs') \<Rightarrow> set (paths (from_list (x#xs'))))"
   unfolding from_list_paths remove_proper_prefixes_def by (cases xs; auto)
 
