Experiments/Test_Suite_Calculation_Refined.thy
@@ -1,0 +1,404 @@
+theory Test_Suite_Calculation_Refined
+  imports Test_Suite_Calculation 
+          "HOL-Library.Product_Lexorder"
+          HOL.Record
+          Deriving.Compare
+          Containers.Containers
+begin
+
+subsection \<open>New Instances\<close>
+
+
+
+
+(* TODO: linear order on FSMs can be created using set_less_aux or similar functions, as all
+         contained sets are finite - but this is probably not that efficient/necessary,
+         as sets of FSMs only occur at one point in the algorithm (collecting ATCs to append
+         after the same path), after which the FSMs are translated to path sets anyway.
+         Still, the instantiation can be made later to profile whether it has any positive
+         effect on performance.
+*)
+instantiation fsm :: (ord,ord,ord) ord
+begin
+
+fun less_eq_fsm ::  "('a,'b,'c) fsm \<Rightarrow> ('a,'b,'c) fsm \<Rightarrow> bool" where
+  "less_eq_fsm M1 M2 = 
+    (if initial M1 < initial M2 
+      then True
+      else ((initial M1 = initial M2) \<and> (if set_less_aux (nodes M1)  (nodes M2)
+        then True
+        else ((nodes M1 = nodes M2) \<and> (if set_less_aux (inputs M1) (inputs M2)
+          then True
+          else ((inputs M1 = inputs M2) \<and> (if set_less_aux (outputs M1) (outputs M2)
+            then True
+            else ((outputs M1 = outputs M2) \<and> (set_less_aux (transitions M1) (transitions M2) \<or> (transitions M1) = (transitions M2))))))))))"
+
+fun less_fsm ::  "('a,'b,'c) fsm \<Rightarrow> ('a,'b,'c) fsm \<Rightarrow> bool" where
+  "less_fsm a b = (a \<le> b \<and> a \<noteq> b)"
+
+instance by (intro_classes)
+end
+
+
+instantiation fsm :: (linorder,linorder,linorder) linorder
+begin
+
+
+
+lemma less_le_not_le_FSM :
+  fixes x :: "('a,'b,'c) fsm"
+  and   y :: "('a,'b,'c) fsm"
+shows "(x < y) = (x \<le> y \<and> \<not> y \<le> x)"
+proof 
+  show "x < y \<Longrightarrow> x \<le> y \<and> \<not> y \<le> x" 
+    
+   
+  proof -
+    assume "x < y"
+    then show "x \<le> y \<and> \<not> y \<le> x"
+    proof (cases "FSM.initial x < FSM.initial y")
+      case True
+      then show ?thesis unfolding less_fsm.simps less_eq_fsm.simps by auto
+    next
+      case False
+      then have *: "FSM.initial x = FSM.initial y"
+        using \<open>x < y\<close> unfolding less_fsm.simps less_eq_fsm.simps by auto
+      
+      show ?thesis proof (cases "set_less_aux (FSM.nodes x) (FSM.nodes y)")
+        case True
+        then show ?thesis 
+          unfolding less_fsm.simps less_eq_fsm.simps 
+          using * set_less_aux_antisym by fastforce
+      next
+        case False
+        then have **: "FSM.nodes x = FSM.nodes y"
+          using \<open>x < y\<close> * unfolding less_fsm.simps less_eq_fsm.simps by auto
+        
+        show ?thesis proof (cases "set_less_aux (FSM.inputs x) (FSM.inputs y)")
+          case True
+          then show ?thesis 
+            unfolding less_fsm.simps less_eq_fsm.simps 
+            using * ** set_less_aux_antisym by fastforce
+        next
+          case False
+          then have ***: "FSM.inputs x = FSM.inputs y"
+            using \<open>x < y\<close> * ** unfolding less_fsm.simps less_eq_fsm.simps by (simp add: set_less_def)
+          
+          show ?thesis proof (cases "set_less_aux (FSM.outputs x) (FSM.outputs y)")
+            case True
+            then show ?thesis 
+              unfolding less_fsm.simps less_eq_fsm.simps 
+              using * ** *** set_less_aux_antisym by fastforce
+          next
+            case False
+            then have ****: "FSM.outputs x = FSM.outputs y"
+              using \<open>x < y\<close> * ** *** unfolding less_fsm.simps less_eq_fsm.simps by (simp add: set_less_def)
+
+
+            have "x \<noteq> y" using \<open>x < y\<close> by auto
+            then have "FSM.transitions x \<noteq> FSM.transitions y"
+              using * ** *** **** by (transfer; auto)
+            then have *****: "set_less_aux (FSM.transitions x) (FSM.transitions y)"
+              using \<open>x < y\<close> * ** *** **** unfolding less_fsm.simps less_eq_fsm.simps by (simp add: set_less_aux_def)
+
+            then have "\<not>(set_less_aux (FSM.transitions y) (FSM.transitions x) \<or> transitions y = transitions x)"
+              using \<open>FSM.transitions x \<noteq> FSM.transitions y\<close> fsm_transitions_finite set_less_aux_antisym by auto
+            then have "\<not> y \<le> x"
+              using * ** *** **** unfolding less_fsm.simps less_eq_fsm.simps 
+              by (simp add: set_less_def)
+            then show ?thesis using \<open>x < y\<close> 
+              using less_fsm.elims(2) by blast
+          qed
+        qed
+      qed
+    qed
+  qed
+
+  show "x \<le> y \<and> \<not> y \<le> x \<Longrightarrow> x < y"
+    using less_fsm.elims(3) by blast
+qed
+
+    
+lemma order_refl_FSM :
+  fixes x :: "('a,'b,'c) fsm"
+  shows "x \<le> x" 
+  by auto
+
+lemma order_trans_FSM :
+  fixes x :: "('a,'b,'c) fsm"
+  fixes y :: "('a,'b,'c) fsm"
+  fixes z :: "('a,'b,'c) fsm"
+  shows "x \<le> y \<Longrightarrow> y \<le> z \<Longrightarrow> x \<le> z"
+  unfolding less_eq_fsm.simps 
+  using less_trans[of "initial x" "initial y" "initial z"]
+        set_less_aux_trans[of "nodes x" "nodes y" "nodes z"]
+        set_less_aux_trans[of "inputs x" "inputs y" "inputs z"]
+        set_less_aux_trans[of "outputs x" "outputs y" "outputs z"]
+        set_less_aux_trans[of "transitions x" "transitions y" "transitions z"]
+  by metis
+
+lemma antisym_FSM :
+  fixes x :: "('a,'b,'c) fsm"
+  fixes y :: "('a,'b,'c) fsm"
+shows "x \<le> y \<Longrightarrow> y \<le> x \<Longrightarrow> x = y"
+  unfolding less_eq_fsm.simps
+  using equal_fsm_def[of x y] 
+  unfolding equal_class.equal
+  by (metis order.asym set_less_aux_antisym)
+
+lemma linear_FSM :
+  fixes x :: "('a,'b,'c) fsm"
+  fixes y :: "('a,'b,'c) fsm"
+shows "x \<le> y \<or> y \<le> x"
+  unfolding less_eq_fsm.simps 
+  by (metis fsm_inputs_finite fsm_nodes_finite fsm_outputs_finite fsm_transitions_finite neq_iff set_less_aux_finite_total) 
+
+
+instance 
+  using less_le_not_le_FSM order_refl_FSM order_trans_FSM antisym_FSM linear_FSM 
+  by (intro_classes; metis+)
+end
+
+
+
+
+instantiation fsm :: (linorder,linorder,linorder) compare
+begin 
+fun compare_fsm :: "('a, 'b, 'c) fsm \<Rightarrow> ('a, 'b, 'c) fsm \<Rightarrow> order" where
+  "compare_fsm x y = comparator_of x y"
+
+instance   
+  using comparator_of compare_fsm.elims
+  by (intro_classes; simp add: comparator_def)
+end
+
+
+instantiation fsm :: (linorder,linorder,linorder) ccompare
+begin
+definition ccompare_fsm :: "(('a, 'b, 'c) fsm \<Rightarrow> ('a, 'b, 'c) fsm \<Rightarrow> order) option" where
+  "ccompare_fsm = Some compare"
+
+instance by (intro_classes; simp add: ccompare_fsm_def comparator_compare)
+end
+
+
+
+subsubsection \<open>Derived Instances\<close>
+
+
+derive (eq) ceq fsm
+
+derive (rbt) set_impl fsm
+derive (rbt) mapping_impl fsm
+
+print_derives
+(*derive (rbt) set_impl sum*)
+(*derive (no) cenum fsm*)
+(*derive (no) cproper_interval sum*)
+
+
+subsection \<open>Updating Code Equations\<close>
+
+subsubsection \<open>New Code Generation for set_as_map\<close>
+
+declare [[code drop: set_as_map]]
+
+lemma set_as_map_code_refined[code] :
+  fixes t :: "('a :: ccompare \<times> 'c :: ccompare) set_rbt" 
+  shows "set_as_map (RBT_set t) = (case ID CCOMPARE(('a \<times> 'c)) of
+           Some _ \<Rightarrow> Mapping.lookup (RBT_Set2.fold (\<lambda> (x,z) m . case Mapping.lookup m (x) of
+                        None \<Rightarrow> Mapping.update (x) {z} m |
+                        Some zs \<Rightarrow> Mapping.update (x) (Set.insert z zs) m)
+                      t
+                      Mapping.empty) |
+           None   \<Rightarrow> Code.abort (STR ''set_as_map RBT_set: ccompare = None'') 
+                                (\<lambda>_. set_as_map (RBT_set t)))"
+proof (cases "ID CCOMPARE(('a \<times> 'c))")
+  case None
+  then show ?thesis by auto
+next
+  case (Some a)
+  
+  let ?f' = "(\<lambda> t' . (RBT_Set2.fold (\<lambda> (x,z) m . case Mapping.lookup m x of
+                                                None \<Rightarrow> Mapping.update x {z} m |
+                                                Some zs \<Rightarrow> Mapping.update x (Set.insert z zs) m)
+                           t'
+                           Mapping.empty))"
+ 
+  let ?f = "\<lambda> xs . (fold (\<lambda> (x,z) m . case Mapping.lookup m x of
+                                                None \<Rightarrow> Mapping.update x {z} m |
+                                                Some zs \<Rightarrow> Mapping.update x (Set.insert z zs) m)
+                          xs Mapping.empty)"
+  have "\<And> xs :: ('a \<times> 'c) list . Mapping.lookup (?f xs) = (\<lambda> x . if (\<exists> z . (x,z) \<in> set xs) then Some {z . (x,z) \<in> set xs} else None)"
+  proof - 
+    fix xs :: "('a \<times> 'c) list"
+    show "Mapping.lookup (?f xs) = (\<lambda> x . if (\<exists> z . (x,z) \<in> set xs) then Some {z . (x,z) \<in> set xs} else None)"
+    proof (induction xs rule: rev_induct)
+      case Nil
+      then show ?case 
+        by (simp add: Mapping.empty.abs_eq Mapping.lookup.abs_eq)
+    next
+      case (snoc xz xs)
+      then obtain x z where "xz = (x,z)" 
+        by (metis (mono_tags, hide_lams) surj_pair)
+  
+      have *: "(?f (xs@[(x,z)])) = (case Mapping.lookup (?f xs) x of
+                                  None \<Rightarrow> Mapping.update x {z} (?f xs) |
+                                  Some zs \<Rightarrow> Mapping.update x (Set.insert z zs) (?f xs))"
+        by auto
+  
+      then show ?case proof (cases "Mapping.lookup (?f xs) x")
+        case None
+        then have **: "Mapping.lookup (?f (xs@[(x,z)])) = Mapping.lookup (Mapping.update x {z} (?f xs))" using * by auto
+  
+        have scheme: "\<And> m k v . Mapping.lookup (Mapping.update k v m) = (\<lambda>k' . if k' = k then Some v else Mapping.lookup m k')"
+          by (metis lookup_update')
+  
+  
+        have m1: "Mapping.lookup (?f (xs@[(x,z)])) = (\<lambda> x' . if x' = x then Some {z} else Mapping.lookup (?f xs) x')"
+          unfolding ** 
+          unfolding scheme by force
+  
+        have "(\<lambda> x . if (\<exists> z . (x,z) \<in> set xs) then Some {z . (x,z) \<in> set xs} else None) x = None"
+        using None snoc by auto
+        then have "\<not>(\<exists> z . (x,z) \<in> set xs)"
+          by (metis (mono_tags, lifting) option.distinct(1))
+        then have "(\<exists> z' . (x,z') \<in> set (xs@[(x,z)]))" and "{z' . (x,z') \<in> set (xs@[(x,z)])} = {z}"
+          by fastforce+
+        then have m2: "(\<lambda> x' . if (\<exists> z' . (x',z') \<in> set (xs@[(x,z)])) then Some {z' . (x',z') \<in> set (xs@[(x,z)])} else None)
+                     = (\<lambda> x' . if x' = x then Some {z} else (\<lambda> x . if (\<exists> z . (x,z) \<in> set xs) then Some {z . (x,z) \<in> set xs} else None) x')"
+          by force
+        
+        show ?thesis using m1 m2 snoc
+          using \<open>xz = (x, z)\<close> by presburger
+      next
+        case (Some zs)
+        then have **: "Mapping.lookup (?f (xs@[(x,z)])) = Mapping.lookup (Mapping.update x (Set.insert z zs) (?f xs))" using * by auto
+        have scheme: "\<And> m k v . Mapping.lookup (Mapping.update k v m) = (\<lambda>k' . if k' = k then Some v else Mapping.lookup m k')"
+          by (metis lookup_update')
+  
+        have m1: "Mapping.lookup (?f (xs@[(x,z)])) = (\<lambda> x' . if x' = x then Some (Set.insert z zs) else Mapping.lookup (?f xs) x')"
+          unfolding ** 
+          unfolding scheme by force
+  
+  
+        have "(\<lambda> x . if (\<exists> z . (x,z) \<in> set xs) then Some {z . (x,z) \<in> set xs} else None) x = Some zs"
+          using Some snoc by auto
+        then have "(\<exists> z' . (x,z') \<in> set xs)"
+          unfolding case_prod_conv using  option.distinct(2) by metis
+        then have "(\<exists> z' . (x,z') \<in> set (xs@[(x,z)]))" by fastforce
+  
+        have "{z' . (x,z') \<in> set (xs@[(x,z)])} = Set.insert z zs"
+        proof -
+          have "Some {z . (x,z) \<in> set xs} = Some zs"
+            using \<open>(\<lambda> x . if (\<exists> z . (x,z) \<in> set xs) then Some {z . (x,z) \<in> set xs} else None) x = Some zs\<close>
+            unfolding case_prod_conv using  option.distinct(2) by metis
+          then have "{z . (x,z) \<in> set xs} = zs" by auto
+          then show ?thesis by auto
+        qed
+  
+        have "\<And> a  . (\<lambda> x' . if (\<exists> z' . (x',z') \<in> set (xs@[(x,z)])) then Some {z' . (x',z') \<in> set (xs@[(x,z)])} else None) a
+                   = (\<lambda> x' . if x' = x then Some (Set.insert z zs) else (\<lambda> x . if (\<exists> z . (x,z) \<in> set xs) then Some {z . (x,z) \<in> set xs} else None) x') a" 
+        proof -
+          fix a show "(\<lambda> x' . if (\<exists> z' . (x',z') \<in> set (xs@[(x,z)])) then Some {z' . (x',z') \<in> set (xs@[(x,z)])} else None) a
+                     = (\<lambda> x' . if x' = x then Some (Set.insert z zs) else (\<lambda> x . if (\<exists> z . (x,z) \<in> set xs) then Some {z . (x,z) \<in> set xs} else None) x') a"
+          using \<open>{z' . (x,z') \<in> set (xs@[(x,z)])} = Set.insert z zs\<close> \<open>(\<exists> z' . (x,z') \<in> set (xs@[(x,z)]))\<close>
+          by (cases "a = x"; auto)
+        qed
+
+        then have m2: "(\<lambda> x' . if (\<exists> z' . (x',z') \<in> set (xs@[(x,z)])) then Some {z' . (x',z') \<in> set (xs@[(x,z)])} else None)
+                     = (\<lambda> x' . if x' = x then Some (Set.insert z zs) else (\<lambda> x . if (\<exists> z . (x,z) \<in> set xs) then Some {z . (x,z) \<in> set xs} else None) x')"
+          by auto
+  
+  
+        show ?thesis using m1 m2 snoc
+          using \<open>xz = (x, z)\<close> by presburger
+      qed
+    qed
+  qed
+  then have "Mapping.lookup (?f' t) = (\<lambda> x . if (\<exists> z . (x,z) \<in> set (RBT_Set2.keys t)) then Some {z . (x,z) \<in> set (RBT_Set2.keys t)} else None)"
+    unfolding fold_conv_fold_keys by metis
+  moreover have "set (RBT_Set2.keys t) = (RBT_set t)" 
+    using Some by (simp add: RBT_set_conv_keys) 
+  ultimately have "Mapping.lookup (?f' t) = (\<lambda> x . if (\<exists> z . (x,z) \<in> (RBT_set t)) then Some {z . (x,z) \<in> (RBT_set t)} else None)"
+    by force
+    
+
+  then show ?thesis 
+    using Some unfolding set_as_map_def by simp
+qed
+
+
+
+subsubsection \<open>New Code Generation for remove_proper_prefixes\<close>
+
+declare [[code drop: remove_proper_prefixes]]
+
+
+lemma remove_proper_prefixes_refined[code] :
+  fixes t :: "('a :: ccompare) list set_rbt" 
+shows "remove_proper_prefixes (RBT_set t) = (case ID CCOMPARE(('a list)) of
+  Some _ \<Rightarrow> (if (is_empty t) then {} else set (paths (from_list (RBT_Set2.keys t)))) |
+  None   \<Rightarrow> Code.abort (STR ''remove_proper_prefixes RBT_set: ccompare = None'') (\<lambda>_. remove_proper_prefixes (RBT_set t)))"
+  (is "?v1 = ?v2")
+proof (cases "ID CCOMPARE(('a list))")
+  case None
+  then show ?thesis by simp
+next
+  case (Some a)
+  then have *:"ID ccompare \<noteq> (None :: ('a::ccompare list \<Rightarrow> 'a::ccompare list \<Rightarrow> order) option)" by auto
+  
+  show ?thesis proof (cases "is_empty t")
+    case True
+    then show ?thesis unfolding Some remove_proper_prefixes_def by auto
+  next
+    case False
+    then have "?v2 = set (paths (from_list (RBT_Set2.keys t)))" using Some by auto
+    moreover have "?v1 = set (paths (from_list (RBT_Set2.keys t)))"
+      using False unfolding RBT_set_conv_keys[OF *, of t] remove_proper_prefixes_code  by (cases "RBT_Set2.keys t"; auto)
+    ultimately show ?thesis by simp
+  qed
+qed
+
+
+subsubsection \<open>New Code Generation for r_distinguishable_state_pairs_with_separators\<close>
+
+declare [[show_types]]
+  declare [[show_sorts]]
+  declare [[show_consts]]
+
+declare [[code drop: r_distinguishable_state_pairs_with_separators]]
+
+value "{(Inr (1::integer,2::integer), Some m_ex_H),(Inr (1,2),Some m_ex_H)} \<union> {(Inl (1::integer,2::integer), Some m_ex_H),(Inr (1,2),Some m_ex_H)}"
+
+lemma r_distinguishable_state_pairs_with_separators_refined[code] :
+  fixes M :: "('a::linorder,'b::linorder,'c::linorder) fsm"
+  shows  "r_distinguishable_state_pairs_with_separators M = (\<Union> q \<in> nodes m_ex_H . {}::(('a \<times> 'a) \<times> (('a \<times> 'a) + 'a,'b,'c) fsm) set)"
+  sorry
+
+
+
+declare pretty_sets[code_post del]
+value "\<Union> q \<in> nodes m_ex_H . nodes m_ex_H"
+value "r_distinguishable_state_pairs_with_separators m_ex_H"
+
+value "{1::integer}"
+
+(*
+lemma r_distinguishable_state_pairs_with_separators_code[code] :
+  "r_distinguishable_state_pairs_with_separators M = 
+    \<Union> (image (\<lambda> ((q1,q2),A) . {((q1,q2),the A),((q2,q1),the A)}) (Set.filter (\<lambda> (qq,A) . A \<noteq> None) (image (\<lambda> (q1,q2) . ((q1,q2),state_separator_from_s_states M q1 q2)) (Set.filter (\<lambda> (q1,q2) . q1 < q2) (nodes M \<times> nodes M)))))"
+  (is "?P1 = ?P2")
+*)
+
+definition ex07 where "ex07 = calculate_test_suite_example_as_io_sequences m_ex_H 4"
+
+
+
+value "calculate_test_suite_example_as_io_sequences m_ex_H 0"
+
+end (*
+export_code ex07 in Haskell module_name FSM2
+
+
+end
