Experiments/Test_Suite_IO.thy
@@ -1438,7 +1438,7 @@ fun test_suite_to_io' :: "('a,'b,'c) fsm \<Rightarrow> ('a,'b,'c,'d) test_suite 
   "test_suite_to_io' M (Test_Suite prs tps rd_targets atcs) = (\<Union> (q,P) \<in> prs . L_acyclic P \<union> (\<Union> ioP \<in> remove_proper_prefixes (L_acyclic P) . \<Union> pt \<in> tps q . ((\<lambda> io' . ioP @ io') ` (set (prefixes (p_io pt)))) \<union> (\<Union> q' \<in> rd_targets (q,pt) . \<Union> (A,t1,t2) \<in> atcs (target q pt,q') . (\<lambda> io_atc . ioP @ p_io pt @ io_atc) ` (acyclic_language_intersection (from_FSM M (target q pt)) A))))"
 
 (* slightly optimized calculation of the test suite representation using only maximal IO-sequences *)
-fun test_suite_to_io'_maximal :: "('a,'b,'c) fsm \<Rightarrow> ('a,'b,'c,'d) test_suite \<Rightarrow> ('b \<times> 'c) list set" where
+fun test_suite_to_io'_maximal :: "('a::linorder,'b::linorder,'c::linorder) fsm \<Rightarrow> ('a,'b,'c,'d::linorder) test_suite \<Rightarrow> ('b \<times> 'c) list set" where
   "test_suite_to_io'_maximal M (Test_Suite prs tps rd_targets atcs) = 
       remove_proper_prefixes (\<Union> (q,P) \<in> prs . L_acyclic P \<union> (\<Union> ioP \<in> remove_proper_prefixes (L_acyclic P) . \<Union> pt \<in> tps q . Set.insert (ioP @ p_io pt) (\<Union> q' \<in> rd_targets (q,pt) . \<Union> (A,t1,t2) \<in> atcs (target q pt,q') . (\<lambda> io_atc . ioP @ p_io pt @ io_atc) ` (remove_proper_prefixes (acyclic_language_intersection (from_FSM M (target q pt)) A)))))"
 
